examples/elliptic/spec/elliptic_exampleScript.sml
@@ -61,65 +61,95 @@ val w2n_lsr = store_thm ("w2n_lsr",
        word_bits_n2w,w2n_n2w,MOD_DIMINDEX,bitTheory.BITS_COMP_THM2]
   ++ SIMP_TAC std_ss [bitTheory.BITS_THM2]);
 
-(* ------------------------------------------------------------------------- *)
-(* Elliptic curve theory to support the compiled functions.                  *)
-(* ------------------------------------------------------------------------- *)
-
-val example_prime_def = Define `example_prime = 751`;
-
-val example_field_def = Define `example_field = GF example_prime`;
-
-val example_curve_def = Define
-  `example_curve = curve example_field 0 0 1 (example_prime - 1) 0`;
-
-val ex_field_elt_def = Define
-  `ex_field_elt (n : num) : word32 = n2w n`;
-
-val ex_field_num_def = Define
-  `ex_field_num (n : num) : word32 = ex_field_elt (n MOD example_prime)`;
-
-val ex_curve_point_def = Define
-  `ex_curve_point =
-   affine_case example_curve (0w,0w) (\x y. (ex_field_elt x, ex_field_elt y))`;
-
 (* ========================================================================= *)
-(* All the below functions need to be compiled.                              *)
+(* Smallest elliptic curve example to be compiled.                           *)
 (* ========================================================================= *)
+
+(* ------------------------------------------------------------------------- *)
+(* First define the parameters for the example using HOL types.              *)
+(* ------------------------------------------------------------------------- *)
+
+val example1_prime_def = Define `example1_prime = 751`;
+
+val example1_field_def = Define `example1_field = GF example1_prime`;
+
+val example1_curve_def = Define
+  `example1_curve = curve example1_field 0 0 1 (example1_prime - 1) 0`;
+
+val example1_elgamal_g_def = Define
+  `example1_elgamal_g = affine example1_field [361; 383]`;
+
+val example1_elgamal_x_def = Define `example1_elgamal_x = 91`;
+
+val example1_elgamal_h_def = Define
+  `example1_elgamal_h =
+   curve_mult example1_curve example1_elgamal_g example1_elgamal_x`;
+
+(* ------------------------------------------------------------------------- *)
+(* Converting HOL types to words.                                            *)
+(* ------------------------------------------------------------------------- *)
+
+val ex1_prime_def = Define `ex1_prime : word32 = n2w example1_prime`;
+
+val ex1_field_elt_def = Define
+  `ex1_field_elt (n : num) : word32 = n2w n`;
+
+val ex1_field_num_def = Define
+  `ex1_field_num (n : num) : word32 = ex1_field_elt (n MOD example1_prime)`;
+
+val ex1_curve_point_def = Define
+  `ex1_curve_point =
+   affine_case example1_curve
+     (0w,0w) (\x y. (ex1_field_elt x, ex1_field_elt y))`;
+
+val ex1_elgamal_g_x = Define
+  `ex1_elgamal_g_x = FST (ex1_curve_point example1_elgamal_g)`;
+
+val ex1_elgamal_g_y = Define
+  `ex1_elgamal_g_y = SND (ex1_curve_point example1_elgamal_g)`;
+
+val ex1_elgamal_h_x = Define
+  `ex1_elgamal_h_x = FST (ex1_curve_point example1_elgamal_h)`;
+
+val ex1_elgamal_h_y = Define
+  `ex1_elgamal_h_y = SND (ex1_curve_point example1_elgamal_h)`;
+
+val ex1_elgamal_x = Define `ex1_elgamal_x = n2w example1_elgamal_x`;
 
 (* ------------------------------------------------------------------------- *)
 (* Representing GF(p) field elements with words.                             *)
 (* ------------------------------------------------------------------------- *)
 
-val ex_field_zero_def = Define
-  `ex_field_zero = ex_field_num 0`;
+val ex1_field_zero_def = Define
+  `ex1_field_zero = ex1_field_num 0`;
 
-val ex_field_neg_def = Define
-  `ex_field_neg (x : word32) =
-   if x = 0w then 0w else n2w example_prime - x`;
+val ex1_field_neg_def = Define
+  `ex1_field_neg (x : word32) =
+   if x = 0w then 0w else ex1_prime - x`;
 
-val ex_field_add_def = Define
-  `ex_field_add (x : word32, y : word32) =
+val ex1_field_add_def = Define
+  `ex1_field_add (x : word32, y : word32) =
    let z = x + y in
-   if z < n2w example_prime then z else z - n2w example_prime`;
+   if z < ex1_prime then z else z - ex1_prime`;
 
-val ex_field_sub_def = Define
-  `ex_field_sub (x : word32, y : word32) =
-   ex_field_add (x, ex_field_neg y)`;
+val ex1_field_sub_def = Define
+  `ex1_field_sub (x : word32, y : word32) =
+   ex1_field_add (x, ex1_field_neg y)`;
 
-val ex_field_mult_def = Define
-  `ex_field_mult (x : word32, y : word32) =
-   word_mod (x * y) (n2w example_prime)`;
+val ex1_field_mult_def = Define
+  `ex1_field_mult (x : word32, y : word32) =
+   word_mod (x * y) (ex1_prime)`;
 
-val (ex_field_exp_aux_def,ex_field_exp_aux_ind) = Defn.tprove
-  (Hol_defn "ex_field_exp_aux"
-   `ex_field_exp_aux (x : word32, n : word32, acc : word32) =
+val (ex1_field_exp_aux_def,ex1_field_exp_aux_ind) = Defn.tprove
+  (Hol_defn "ex1_field_exp_aux"
+   `ex1_field_exp_aux (x : word32, n : word32, acc : word32) =
     if n = 0w then acc
     else
-      let x' = ex_field_mult (x,x) in
+      let x' = ex1_field_mult (x,x) in
       let n' = n >>> 1 in
-      let acc' = if n && 1w = 0w then acc else ex_field_mult (acc,x) in
-      ex_field_exp_aux (x',n',acc')`,
-   WF_REL_TAC `measure (\(x,y,z). w2n y)`
+      let acc' = if n && 1w = 0w then acc else ex1_field_mult (acc,x) in
+      ex1_field_exp_aux (x',n',acc')`,
+   WF_REL_TAC `measure (\(x,n,a). w2n n)`
    ++ RW_TAC arith_ss [w2n_lsr]
    ++ Know `~(w2n n = 0)` >> METIS_TAC [n2w_w2n]
    ++ Q.SPEC_TAC (`w2n n`,`n`)
@@ -129,55 +159,55 @@ val (ex_field_exp_aux_def,ex_field_exp_aux_ind) = Defn.tprove
    >> PROVE_TAC [TWO, ellipticTheory.DIV_THEN_MULT]
    ++ DECIDE_TAC);
 
-val ex_field_exp_def = Define
-  `ex_field_exp (x : word32, n : word32) = ex_field_exp_aux (x,n,1w)`;
+val ex1_field_exp_def = Define
+  `ex1_field_exp (x : word32, n : word32) = ex1_field_exp_aux (x,n,1w)`;
 
-val ex_field_inv_def = Define
-  `ex_field_inv (x : word32) =
-   ex_field_exp (x, n2w (example_prime - 2))`;
+val ex1_field_inv_def = Define
+  `ex1_field_inv (x : word32) =
+   ex1_field_exp (x, n2w (example1_prime - 2))`;
 
-val ex_field_div_def = Define
-  `ex_field_div (x : word32, y : word32) =
-   ex_field_mult (x, ex_field_inv y)`;
+val ex1_field_div_def = Define
+  `ex1_field_div (x : word32, y : word32) =
+   ex1_field_mult (x, ex1_field_inv y)`;
 
 (* ------------------------------------------------------------------------- *)
 (* Elliptic curve operations in terms of the above field operations.         *)
 (* ------------------------------------------------------------------------- *)
 
-val ex_curve_zero_def = Define
-  `ex_curve_zero = ex_curve_point (curve_zero example_curve)`;
+val ex1_curve_zero_def = Define
+  `ex1_curve_zero = ex1_curve_point (curve_zero example1_curve)`;
 
-val ex_curve_neg_def = Define
-  `ex_curve_neg (x1,y1) =
-   let $~ = ex_field_neg in
-   let $- = CURRY ex_field_sub in
-   let $* = CURRY ex_field_mult in
-   let a1 = ex_field_elt example_curve.a1 in
-   let a3 = ex_field_elt example_curve.a3 in
-   if (x1,y1) = ex_curve_zero then ex_curve_zero
+val ex1_curve_neg_def = Define
+  `ex1_curve_neg (x1,y1) =
+   let $~ = ex1_field_neg in
+   let $- = CURRY ex1_field_sub in
+   let $* = CURRY ex1_field_mult in
+   let a1 = ex1_field_elt example1_curve.a1 in
+   let a3 = ex1_field_elt example1_curve.a3 in
+   if (x1,y1) = ex1_curve_zero then ex1_curve_zero
    else
      let x = x1 in
      let y = ~y1 - a1 * x1 - a3 in
      (x,y)`;
 
-val ex_curve_double_def = Define
-  `ex_curve_double (x1,y1) =
-   let $& = ex_field_num in
-   let $~ = ex_field_neg in
-   let $+ = CURRY ex_field_add in
-   let $- = CURRY ex_field_sub in
-   let $* = CURRY ex_field_mult in
-   let $/ = CURRY ex_field_div in
-   let $** = CURRY ex_field_exp in
-   let a1 = ex_field_elt example_curve.a1 in
-   let a2 = ex_field_elt example_curve.a2 in
-   let a3 = ex_field_elt example_curve.a3 in
-   let a4 = ex_field_elt example_curve.a4 in
-   let a6 = ex_field_elt example_curve.a6 in
-   if (x1,y1) = ex_curve_zero then ex_curve_zero
+val ex1_curve_double_def = Define
+  `ex1_curve_double (x1,y1) =
+   let $& = ex1_field_num in
+   let $~ = ex1_field_neg in
+   let $+ = CURRY ex1_field_add in
+   let $- = CURRY ex1_field_sub in
+   let $* = CURRY ex1_field_mult in
+   let $/ = CURRY ex1_field_div in
+   let $** = CURRY ex1_field_exp in
+   let a1 = ex1_field_elt example1_curve.a1 in
+   let a2 = ex1_field_elt example1_curve.a2 in
+   let a3 = ex1_field_elt example1_curve.a3 in
+   let a4 = ex1_field_elt example1_curve.a4 in
+   let a6 = ex1_field_elt example1_curve.a6 in
+   if (x1,y1) = ex1_curve_zero then ex1_curve_zero
    else
      let d = & 2 * y1 + a1 * x1 + a3 in
-     if d = ex_field_zero then ex_curve_zero
+     if d = ex1_field_zero then ex1_curve_zero
      else
        let l = (& 3 * x1 ** 2w + & 2 * a2 * x1 + a4 - a1 * y1) / d in
        let m = (~(x1 ** 3w) + a4 * x1 + & 2 * a6 - a3 * y1) / d in
@@ -185,25 +215,25 @@ val ex_curve_double_def = Define
        let y = ~(l + a1) * x - m - a3 in
        (x,y)`;
 
-val curve_add_def = Define
-  `curve_add (x1,y1,x2,y2) =
-   if (x1 = x2) /\ (y1 = y2) then ex_curve_double (x1,y1)
+val ex1_curve_add_def = Define
+  `ex1_curve_add (x1,y1,x2,y2) =
+   if (x1 = x2) /\ (y1 = y2) then ex1_curve_double (x1,y1)
    else
-     let $& = ex_field_num in
-     let $~ = ex_field_neg in
-     let $+ = CURRY ex_field_add in
-     let $- = CURRY ex_field_sub in
-     let $* = CURRY ex_field_mult in
-     let $/ = CURRY ex_field_div in
-     let $** = CURRY ex_field_exp in
-     let a1 = ex_field_elt example_curve.a1 in
-     let a2 = ex_field_elt example_curve.a2 in
-     let a3 = ex_field_elt example_curve.a3 in
-     let a4 = ex_field_elt example_curve.a4 in
-     let a6 = ex_field_elt example_curve.a6 in
-     if (x1,y1) = ex_curve_zero then (x2,y2)
-     else if (x2,y2) = ex_curve_zero then (x1,y1)
-     else if x1 = x2 then ex_curve_zero
+     let $& = ex1_field_num in
+     let $~ = ex1_field_neg in
+     let $+ = CURRY ex1_field_add in
+     let $- = CURRY ex1_field_sub in
+     let $* = CURRY ex1_field_mult in
+     let $/ = CURRY ex1_field_div in
+     let $** = CURRY ex1_field_exp in
+     let a1 = ex1_field_elt example1_curve.a1 in
+     let a2 = ex1_field_elt example1_curve.a2 in
+     let a3 = ex1_field_elt example1_curve.a3 in
+     let a4 = ex1_field_elt example1_curve.a4 in
+     let a6 = ex1_field_elt example1_curve.a6 in
+     if (x1,y1) = ex1_curve_zero then (x2,y2)
+     else if (x2,y2) = ex1_curve_zero then (x1,y1)
+     else if x1 = x2 then ex1_curve_zero
      else
        let d = x2 - x1 in
        let l = (y2 - y1) / d in
@@ -211,5 +241,78 @@ val curve_add_def = Define
        let x = l ** 2w + a1 * l - a2 - x1 - x2 in
        let y = ~(l + a1) * x - m - a3 in
        (x,y)`;
+
+val (ex1_curve_mult_aux_def,ex1_curve_mult_aux_ind) = Defn.tprove
+  (Hol_defn "ex1_curve_mult_aux"
+   `ex1_curve_mult_aux (x : word32, y : word32, n : word32,
+                       acc_x : word32, acc_y : word32) =
+    if n = 0w then (acc_x,acc_y)
+    else
+      let (x',y') = ex1_curve_double (x,y) in
+      let n' = n >>> 1 in
+      let (acc_x',acc_y') = if n && 1w = 0w then (acc_x,acc_y)
+                            else ex1_curve_add (x,y,acc_x,acc_y) in
+      ex1_curve_mult_aux (x',y',n',acc_x',acc_y')`,
+   WF_REL_TAC `measure (\(x,y,n,xa,ya). w2n n)`
+   ++ RW_TAC arith_ss [w2n_lsr]
+   ++ Know `~(w2n n = 0)` >> METIS_TAC [n2w_w2n]
+   ++ Q.SPEC_TAC (`w2n n`,`n`)
+   ++ POP_ASSUM_LIST (K ALL_TAC)
+   ++ RW_TAC arith_ss []
+   ++ Know `2 * (n DIV 2) <= n`
+   >> PROVE_TAC [TWO, ellipticTheory.DIV_THEN_MULT]
+   ++ DECIDE_TAC);
+
+val ex1_curve_mult_def = Define
+  `ex1_curve_mult (x : word32, y : word32, n : word32) =
+   ex1_curve_mult_aux (x,y,n,0w,0w)`;
+
+(* ------------------------------------------------------------------------- *)
+(* Elliptic curve encryption and decryption functions.                       *)
+(* These form the API, and need to be compiled.                              *)
+(* ------------------------------------------------------------------------- *)
+
+val ex1_elgamal_encrypt_def = Define
+  `ex1_elgamal_encrypt (m_x : word32, m_y : word32, k : word32) =
+   let (a_x,a_y) = ex1_curve_mult (ex1_elgamal_g_x,ex1_elgamal_g_y,k) in
+   let (t_x,t_y) = ex1_curve_mult (ex1_elgamal_h_x,ex1_elgamal_h_y,k) in
+   let (b_x,b_y) = ex1_curve_add (t_x,t_y,m_x,m_y) in
+   (a_x,a_y,b_x,b_y)`;
+
+val elgamal_decrypt_def = Define
+  `elgamal_decrypt (a_x,a_y,b_x,b_y) =
+   let (t_x,t_y) = ex1_curve_neg (ex1_curve_mult (a_x,b_x,ex1_elgamal_x)) in
+   ex1_curve_add (t_x,t_y,b_x,b_y)`;
+
+(* ========================================================================= *)
+(* A multiword elliptic curve example to be compiled.                        *)
+(* ========================================================================= *)
+
+(* ------------------------------------------------------------------------- *)
+(* First define the parameters for the example using HOL types.              *)
+(* ------------------------------------------------------------------------- *)
+
+val example2_prime_def = Define `example2_prime = 751`;
+
+val example2_field_def = Define `example2_field = GF example2_prime`;
+
+(* ------------------------------------------------------------------------- *)
+(* Converting HOL types to words.                                            *)
+(* ------------------------------------------------------------------------- *)
+
+val ex2_prime0 = Define
+  `ex2_prime0 : word32 = n2w example2_prime`;
+
+val ex2_prime1 = Define
+  `ex2_prime1 : word32 = n2w (example2_prime DIV 2 ** 32)`;
+
+val ex2_field_neg_def = Define
+  `ex2_field_neg (x0 : word32, x1 : word32) =
+   if (x0 = 0w) /\ (x1 = 0w) then (0w,0w)
+   else
+     let y0 = ex2_prime0 - x0 in
+     let y1 = if y0 <= ex2_prime0 then ex2_prime1 - x1
+              else ex2_prime1 - (x1 + 1w) in
+     (y0,y1)`;
 
 val () = export_theory ();
